\begin{enumerate}[label=(\alph*)]
\item From the student's perspective, the average class size is $\text{E}(X)
=
\frac{200}{360}100 + \frac{160}{360}10 = 60$. From the dean's perspective, the
average class size is $\text{E}(X) = \frac{16}{18}10 + \frac{2}{18}100 =
20$. The discrepancy comes from the fact that when surveying the dean, there are
only two data points with a large number of students. However, when surveying
students, there are two hundred data points with a large number of students.
In a sense, the student's perspective overcounts the classes.

\item Let the university consist of classes of size \(c_{1}, c_{2},...,c_{k}\), of which there are \(n_{1}\) classes of size \(c_{1}\), \(n_{2}\) classes of size \(c_{2}\), etc, up to \(n_{k}\) classes of size \(c_{k}\). \\

Let N be the total number of classes, with \(N = \sum\limits_{i=1}^{i=k}n_{i}\), and P be the total population of the university, with \(P = \sum\limits_{i=1}^{i=k}n_{i}c_{i}\).\\

Let \(X\) be the number of students in a random class. Let \(Y\) be the size of a random student's class.\\

We have \textbf{Equation 1: }\(E(X) = \sum\limits_{i=1}^{i=k}\frac{n_{i}}{N}c_{i}\).\\

We also have \textbf{Equation 2: }\(E(Y) = \sum\limits_{i=1}^{i=k}\frac{n_{i}*c_{i}}{P}c_{i}\). \\

We must prove \(E(X) >= E(Y)\).\\

Since variance is non-negative, we know \(E(X^{2}) \geq (E(X))^{2}\). This will give us

\[\sum\limits_{i=1}^{i=k}\frac{n_{i}}{N}c_{i}^{2} \geq (\sum\limits_{i=1}^{i=k}\frac{n_{i}}{N}c_{i})^2\]\\

Noting that N is a constant, and noting that \(\sum\limits_{i=1}^{i=k}n_{i}c_{i}=P\), this rearranges to \textbf{Inequality 3: }\[N*\sum\limits_{i=1}^{i=k}(n_{i}c_{i}^{2}) \geq P*\sum\limits_{i=1}^{i=k}(n_{i}c_{i})\]

If we divide both sides by \(N*P\) and then compare to Equations 1 and 2, we realize that Inequality 3 is equivalent to \(E(X) \geq E(Y)\). \\

Next, we shall prove that equality only occurs if all the \(c_{i}\) are equal. If we expand \(N\) and \(P\) in Inequality 3 and expand out terms, we get:

\[\sum\limits_{i=1}^{i=k}(n_{i}^{2}c_{i}^{2}) + \sum\limits_{i\neq j}(n_{i}n_{j}c_{i}^{2}) \geq \sum\limits_{i=1}^{i=k}(n_{i}^{2}c_{i}^{2}) + \sum\limits_{i\neq j}(n_{i}n_{j}c_{i}c_{j})\]

which simplifies to:

\[\sum\limits_{i\neq j}(n_{i}n_{j}c_{i}^{2}) \geq \sum\limits_{i\neq j}(n_{i}n_{j}c_{i}c_{j})\]

Subtracting the right side from both sides of the equation, we observe that this is equivalent to:

\[\sum\limits_{i\neq j}(n_{i}n_{j}(c_{i}-c_{j})^{2}) \geq 0\]

Assuming that the \(n_{i},n_{j}\) are positive, equality only holds here if \(c_{i}=c_{j}\) for all distinct \(i,j\), concluding our proof. 

\end{enumerate}
