(a)
\begin{equation*}
\begin{split}
\Phi(z)
&= \frac{1}{\sqrt{2\pi}} \int_{-\infty}^z e^{-x^2/2} dx \\
&= \frac{1}{\sqrt{2\pi}} \left( \int_{-\infty}^0 e^{-x^2/2} dx + \int_0^z e^{-x^2/2} dx \right)
\end{split}
\end{equation*}

We know from the Normal PDF that $\int_{-\infty}^{\infty} e^{-x^2/2} dx = \sqrt{2\pi}$. Since the integrand is an even function, the integral from $-\infty$ to $0$ is half this value

$$
\Phi(z) = \frac{1}{2} + \frac{1}{\sqrt{2\pi}} \int_0^z e^{-x^2/2} dx
$$

By applying the variable substitution $u = x/\sqrt{2}$ in the integral, we obtain $du = dx/\sqrt{2}$. The lower and upper limits of integration become $0$ and $z/\sqrt{2}$, respectively.

\begin{equation*}
\begin{split}
\Phi(z)
&= \frac{1}{2} + \frac{1}{\sqrt{2\pi}} \int_0^{z/\sqrt{2}} e^{-u^2} \sqrt{2} \, du \\
&= \frac{1}{2} + \frac{1}{2} \frac{2}{\sqrt{\pi}} \int_0^{z/\sqrt{2}} e^{-u^2} du
\end{split}
\end{equation*}

$$
\Phi(z) = \frac{1}{2} + \frac{1}{2} \, \mathrm{erf} \left( \frac{z}{\sqrt{2}} \right)
$$


(b)
$$
\mathrm{erf}(z) = \frac{2}{\sqrt{\pi}} \int_0^z e^{-x^2} dx
$$

The integrand is an even function, so the integrals from 0 to $z$ and from $-z$ to 0 are the same

\begin{equation*}
\begin{split}
\mathrm{erf}(z)
&= \frac{2}{\sqrt{\pi}} \int_{-z}^0 e^{-x^2} dx \\
&= - \frac{2}{\sqrt{\pi}} \int_0^{-z} e^{-x^2} dx
\end{split}
\end{equation*}

$$
\mathrm{erf}(-z) = -\mathrm{erf}(z)
$$
