\begin{enumerate}[label=(\alph*)]
\item $P(X=k) = \binom{n}{k}p^{k}(1-p)^{n-k}$ for $0 \leq k \leq 3$.

\item To use the complement of the desired deven, $$P(X > 0) = 1 - P(X = 0) = 1 -
(1- p)^{3} = 1 - (-p^{3} + 3p^{2} - 3p + 1) = p^{3} - 3p^{2} + 3p.$$

To prove the same by Inclusion-Exclusion,

$$P(X > 0) = \sum_{i=1}^{3} P(I_{X_{i}}=1) - 3p^{2} + P(\cap_{i=1}^{3}I_{X_
{i}} =
1) = 3p -3p^{2} + p^{3}.$$

\item Since $p^{2}$ and $p^{3}$ go to $0$ asymptotically faster than $p$, when
$p$ is small, $3p - 3p^{2} + p^{3} \approx 3p$.
\end{enumerate}