Let $D$ be the event that a person has the disease. Let $T$ be the event
that a person tests positive for the disease.

\begin{enumerate}[label=(\alph*)]
\item 
\begin{align*}
P(D|T) &= \frac{P(D)P(T|D)}{P(T)} \\
&= \frac{p(P(A|D)P(T|D, A) + P(B|D)P(T|D, B))}{P(A)P(T|A) + P(B)P(T|B)} \\
&= \frac{p\left(\frac{1}{2}a_{1} + \frac{1}{2}b_{1}\right)}{\frac{1}{2}\left
(P(D|A)P(T|D, A) + P(D^{c}|A)P(T|D^{c}, A)\right) + \frac{1}{2}\left(P
(D|B)P(T|D, B) + P(D^{c}|B)P(T|D^{c}, B)\right)} \\
&= \frac{\frac{1}{2}p(a_{1} + b_{1})}{\frac{1}{2}(pa_{1} + (1-p)(1-a_{2})) +
\frac{1}{2}(pb_{1} + (1-p)(1-b_{2}))}
\end{align*}

\item
\begin{align*}
P(A|T) &= \frac{P(A)P(T|A)}{P(T)} \\
&= \frac{\frac{1}{2}(pa_{1} + (1-p)(1-a_{2}))}{P(A)P(T|A) + P(B)P(T|B)} \\
&= \frac{\frac{1}{2}(pa_{1} + (1-p)(1-a_{2}))}{\frac{1}{2}(pa_{1} + (1-p)(1-a_
{2})) + \frac{1}{2}(pb_{1} + (1-p)(1-b_{2}))}
\end{align*}
\end{enumerate}