\begin{enumerate}[label=(\alph*)]
\item 
\begin{align*}
P(D|\bigcap\limits^n_{i=1}T_{i}) &= \frac{P(D)P(\bigcap\limits^n_{i=1}T_{i}|D)}
{P(\bigcap\limits^n_{i=1}T_{i})} \\
&= \frac{p\prod_{i=1}^{n} a}{p\prod_{i=1}^{n} a + q\prod_{i=1}^{n} b} \\
&= \frac{pa^{n}}{pa^{n} + qb^{n}}
\end{align*}

\item
\begin{align*}
P(D|\bigcap\limits^n_{i=1}T_{i}) &= \frac{P(D)P(\bigcap\limits^n_{i=1}T_{i}|D)}
{P(\bigcap\limits^n_{i=1}T_{i})} \\
&= \frac{p(P(G)P(\bigcap\limits^n_{i=1}T_{i}|D, G) + P(G^{c})P(\bigcap\limits^n_
{i=1}T_{i}|D, G^{c}))}{P(\bigcap\limits^n_{i=1}T_{i})} \\
&= \frac{p(\frac{1}{2} + \frac{1}{2}a_{0}^{n})}{P(G)P(\bigcap\limits^n_
{i=1}T_{i}|G) + P(G^{c})P(\bigcap\limits^n_{i=1}T_{i}|G^{c})} \\
&= \frac{p(\frac{1}{2} + \frac{1}{2}a_{0}^{n})}{P(G)(P(D|G)P(\bigcap\limits^n_
{i=1}T_{i}|D, G) + P(D^{c}|G)P(\bigcap\limits^n_{i=1}T_{i}|D^{c}, G)) + P(G^{c})
(P(D|G^{c})P(\bigcap\limits^n_{i=1}T_{i}|D, G^{c}) + P(D^{c}|G^{c})P
(\bigcap\limits^n_{i=1}T_{i}|D^{c}, G^{c}))} \\
&= \frac{p(\frac{1}{2} + \frac{1}{2}a_{0}^{n})}{\frac{1}{2} + \frac{1}{2}(pa_
{0}^{n} + (1-p)b_{0}^{n})} \\
&= \frac{p(1 + a_{0}^{n})}{1 + pa_{0}^{n} + (1-p)b_{0}^{n}}
\end{align*}
\end{enumerate}