\begin{enumerate}[label=(\alph*)]
\item To have $j$ toy types after sampling $i$ toys, we either have $j-1$ toy types after sampling $i-1$ toys, and the $i$-th toy is of a previously unseen type, or, we have $j$ toy types after sampling $i-1$ toys, and the $i$-th toy has an already seen type.

Thus, $$p_{i,j} = p_{i-1,j-1} \frac{n-j+1}{n} + p_{i-1,j} \frac{j}{n}$$

\item Note that $p_{1,0} = 0, p_{1, 1} = 1$ and $p_{i, j} = 0$ for $j > i$. Using strong induction, a proof of the recursion in part $a$ follows.
\end{enumerate}
