\begin{enumerate}[label=(\alph*)]
\item 
$$p_{n} = a_{n}a + (1-a_{n})b = (a - b)a_{n} + b$$

$$a_{n+1} = a_{n}a + (1-a_{n})(1-b) = a_{n}(a + b - 1) + 1 - b$$

\item $$p_{n+1} = (a-b)a_{n+1} + b$$
$$p_{n+1} = (a-b)((a + b - 1)a_{n} + 1 - b) + b$$
$$p_{n+1} = (a-b)\left((a + b - 1)\frac{p_{n} - b}{a - b} + 1 - b\right) + b$$
$$p_{n+1} = (a + b - 1)p_{n} + a + b - 2ab$$

\item Let $p = \lim_{n \to \infty} p_{n}$. Taking the limit of both sides of the result of part $b$, we get 
$$p = (a + b - 1)p + a + b - 2ab$$
$$p = \frac{a + b - 2ab}{2 - (a + b)}$$
\end{enumerate}

