Let \(g(Z) = max(Z-c, 0)\). We have \(g(Z) = 0\) for \(Z < c\) and \(g(Z) = Z-c\) for \(Z>c\).\\

Then 

\[E(g(Z)) = \int_{-\infty}^{\infty}g(k)\varphi(k)dk = \int_{c}^{\infty}(k-c)\varphi(k)dk\]

since the expression inside the integral is 0 for \(k<c\). Next we have

\[\int_{c}^{\infty}(k-c)\varphi(k)dk = \int_{c}^{\infty}\frac{ke^{-k^{2}/2}}{\sqrt{2\pi}}dk  - \int_{c}^{\infty}c\varphi(k)dk = \frac{e^{-c^{2}/2}}{\sqrt{2\pi}} - c\int_{-\infty}^{-c}\varphi(k) = \varphi(c) - c\Phi(c)\]

with the first equality following from splitting the integral via subtraction and expanding out \(\varphi\) for the left integral, the second equality comes from observing that the antiderivative of \(k\varphi(k)\) is \(-\varphi(k)\) and that we can change the limits of the right integral due to the symmetry of tail areas of the curve of \(\varphi\), and the last equality comes from applying the definitions of the PDF and CDF of the standard normal distribution.
