a. Let's develop the integral $\int_0^t h(s) ds$

$$
\int_0^t h(s) ds = \int_0^t \frac{f(s)}{1 - F(s)} ds = \int_0^t \frac{f(s)}{G(s)} ds
$$

\noindent where $G(t) = 1 - F(t)$ is the survival function.


Doing the substitution $v = \log G(s)$, we have

$$
dv = \frac{G\;\!'(s)}{G(s)} ds = -\, \frac{F\;\!'(s)}{G(s)} ds = -\, \frac{f(s)}{G(s)} ds
$$


With the substitution, the lower limit of integration becomes $\log G(0) = \log 1 = 0$, and the upper limit becomes $\log G(t)$.
Therefore,

\begin{equation} \label{eq_h_G}
\int_0^t h(s) ds = \int_0^{\log G(t)} - dv = -\log G(t)
\end{equation}


$$
\log G(t) = - \int_0^t h(s) ds
$$

$$
G(t) = 1 - F(t) = \exp \left( - \int_0^t h(s) ds \right)
$$

$$
F(t) = 1 - \exp \left( - \int_0^t h(s) ds \right) \text{ , for all } t>0
$$ \\


b. The PDF is the derivative of the CDF

$$
f(t) = F\;\!'(t) = \left[ 1 - \exp \left( - \int_0^t h(s) ds \right) \right]'
$$

\begin{equation} \label{eq_f_expint}
f(t) = - \exp \left( - \int_0^t h(s) ds \right) \cdot \left( - \int_0^t h(s) ds \right)'
\end{equation}

To calculate the derivative of the integral in the relation above, let's apply the differential in both sides of equation \eqref{eq_h_G}

$$
\left( \int_0^t h(s) ds \right)'
=
\left( - \log G(t) \right)'
=
- \frac{G\;\!'(t)}{G(t)}
=
\frac{ (F(t)-1)' }{G(t)}
=
\frac{f(t)}{1 - F(t)}
=
h(t)
$$

Substituting this result in equation \eqref{eq_f_expint}

$$
f(t) = - \exp \left( - \int_0^t h(s) ds \right) \cdot (-h(t))
$$

$$
f(t) = h(t) \exp \left( - \int_0^t h(s) ds \right) \text{ , for all } t>0
$$
