\begin{enumerate}[label=(\alph*)]

\item Since the trials are independent, the probability that the first $k-1$
trials fail is $(\frac{1}{2})^{k-1}$, and the probability that the 
$k$-th trial is successful is $\frac{1}{2}$. Thus, for $k \geq 1$,

$$P(X=k) = (\frac{1}{2})^{k-1}*\frac{1}{2}.$$

\item This problem reduces to part $a$ once a trial is performed. Whatever it's
outcome, we label it failure and proceed to perform more trials until the
opposite outcome is observed. Thus, for $k \geq 2$,

$$P(X=k) = (\frac{1}{2})^{k-2} * \frac{1}{2}.$$


\end{enumerate}