\begin{enumerate}[label=(\alph*)]

\item 
If $A$ and $B$ are independent, then 
$$P(A|B, C) = P(A|B^{c}, C) = P(A|C).$$
$$P(A|B, C^{c}) = P(A|B^{c}, C^{c}) = P(A|C^{c}).$$

Thus, Simpson's Paradox does not hold.

\item
If $A$ and $C$ are independent, then $P(A|B, C) < P(A|B^{c}, C) \implies P(A|B)
< P(A|B^{c}).$ Thus, Simpson's Paradox does not hold.

\item
If $B$ and $C$ are independent, then
$$P(A|B) = P(C)P(A|B, C) + P(C^{c})P(A|B, C^{c}).$$
$$P(A|B^{c}) = P(C)P(A|B^{c}, C) + P(C^{c})P(A|B^{c}, C^{c}).$$

Since $P(A|B, C) > P(A|B^{c}, C)$ and $P(A|B, C^{c}) > P(A|B^{c}, C^{c})$, $P
(A|B) > P(A|B^{c})$, so Simpson's Paradox does not hold.
\end{enumerate}